proofs/core/Alpha.v
@@ -1,5 +1,6 @@
 Require Export SubMulti.
 Require Import GenElts.
+Require Import PatternProofs.
 
 (*For a proof using induction on length of list*)
 Require Import Coq.Arith.Wf_nat.
@@ -127,11 +128,11 @@ Ltac alpha_case x Heq :=
 Section Alpha.
 
 Context {gamma: context} (gamma_valid: valid_context gamma)
- {pd: pi_dom}
-  {vt: val_typevar} {pf: pi_funpred gamma_valid pd}.
+ {pd: pi_dom} {pdf: pi_dom_full gamma pd}
+  {vt: val_typevar} {pf: pi_funpred gamma_valid pd pdf}.
 
-Notation term_rep := (term_rep gamma_valid pd vt pf).
-Notation formula_rep := (formula_rep gamma_valid pd vt pf).
+Notation term_rep := (term_rep gamma_valid pd pdf vt pf).
+Notation formula_rep := (formula_rep gamma_valid pd pdf vt pf).
 
 (*Check that (x, y) binding is at the same point in the list.*)
 Definition eq_var (vars: list (vsymbol * vsymbol)) v1 v2 :=
@@ -745,11 +746,11 @@ Lemma match_val_single_alpha_p_none {ty: vty}
 (p1 p2: pattern)
 (Hty1: pattern_has_type gamma p1 ty)
 (Hty2: pattern_has_type gamma p2 ty)
-(d: domain (dom_aux pd) (v_subst vt ty))
+(d: domain pd (v_subst vt ty))
 (vars: list (vsymbol * vsymbol))
 (Heq: alpha_equiv_p vars p1 p2) :
-match_val_single gamma_valid pd vt ty p1 Hty1 d = None ->
-match_val_single gamma_valid pd vt ty p2 Hty2 d = None.
+match_val_single gamma_valid pd pdf vt ty p1 Hty1 d = None ->
+match_val_single gamma_valid pd pdf vt ty p2 Hty2 d = None.
 Proof.
   revert ty d Hty1 Hty2.
   generalize dependent p2. induction p1.
@@ -983,11 +984,11 @@ Lemma match_val_single_alpha_p_none_iff {ty: vty}
   (p1 p2: pattern)
   (Hty1: pattern_has_type gamma p1 ty)
   (Hty2: pattern_has_type gamma p2 ty)
-  (d: domain (dom_aux pd) (v_subst vt ty))
+  (d: domain pd (v_subst vt ty))
   (vars: list (vsymbol * vsymbol))
   (Heq: alpha_equiv_p vars p1 p2):
-  match_val_single gamma_valid pd vt ty p1 Hty1 d = None <->
-  match_val_single gamma_valid pd vt ty p2 Hty2 d = None.
+  match_val_single gamma_valid pd pdf vt ty p1 Hty1 d = None <->
+  match_val_single gamma_valid pd pdf vt ty p2 Hty2 d = None.
 Proof.
   split; intros.
   - apply (match_val_single_alpha_p_none p1 p2 Hty1 _ _ _ Heq); auto.
@@ -1002,14 +1003,14 @@ Lemma match_val_single_alpha_p_some {ty: vty}
   (p1 p2: pattern)
   (Hty1: pattern_has_type gamma p1 ty)
   (Hty2: pattern_has_type gamma p2 ty)
-  (d: domain (dom_aux pd) (v_subst vt ty))
+  (d: domain pd (v_subst vt ty))
   (vars: list (vsymbol * vsymbol))
   (Heq: alpha_equiv_p vars p1 p2)
   (Hnodup1: NoDup (map fst vars))
   (Hnodup2: NoDup (map snd vars))
   l1 l2 x y t (def: vsymbol):
-  match_val_single gamma_valid pd vt ty p1 Hty1 d = Some l1 ->
-  match_val_single gamma_valid pd vt ty p2 Hty2 d = Some l2 ->
+  match_val_single gamma_valid pd pdf vt ty p1 Hty1 d = Some l1 ->
+  match_val_single gamma_valid pd pdf vt ty p2 Hty2 d = Some l2 ->
   In (x, y) vars ->
   In (x, t) l1 <-> In (y, t) l2.
 Proof.
@@ -1281,7 +1282,7 @@ Proof.
     rewrite <- (H _ _ v1 v2 _ Hty1 Hty2 Htm) at 1; auto.
     
     (*Now need to know [match_val_single] is same - separate lemmas*)
-    destruct ( match_val_single gamma_valid pd vt tys2 p1 (Forall_inv Hpat1)
+    destruct ( match_val_single gamma_valid pd pdf vt tys2 p1 (Forall_inv Hpat1)
     (term_rep v1 tm tys2 Hty1)) eqn : Hmatch1.
     + (*In Some case, need to know how lists relate*)
 
@@ -1291,7 +1292,7 @@ Proof.
         bool_hyps; auto.
       }
       pose proof (alpha_equiv_p_fv_len_full _ _ Hpeq) as Hlen2.
-      destruct (  match_val_single gamma_valid pd vt tys2 p2 (Forall_inv Hpat2)
+      destruct (  match_val_single gamma_valid pd pdf vt tys2 p2 (Forall_inv Hpat2)
       (term_rep v1 tm tys2 Hty1)) eqn : Hmatch2.
       * assert (A:=Hall). specialize (A 0 ltac:(lia)); simpl in A.
         bool_hyps. rename H1 into Hp; rename H3 into Ht12.
@@ -1312,7 +1313,7 @@ Proof.
             (*Now, we know that x is in l by 
               [match_val_single_free_var]*)
             assert (Hinxl: In x (map fst l)). {
-              apply (match_val_single_free_var _ _ _ _ _ _ _ _ x) in Hmatch1.
+              apply (match_val_single_free_var _ _ _ _ _ _ _ _ _ x) in Hmatch1.
               auto.
               apply Hmatch1. subst. wf_tac.
             }
@@ -1391,7 +1392,7 @@ Proof.
         rewrite <- match_val_single_alpha_p_none_iff in Hmatch2.
         rewrite Hmatch2 in Hmatch1. inversion Hmatch1. apply Hpeq.
     + (*In None case, both None, use IH*) 
-      assert (match_val_single gamma_valid pd vt tys2 p2 (Forall_inv Hpat2)
+      assert (match_val_single gamma_valid pd pdf vt tys2 p2 (Forall_inv Hpat2)
       (term_rep v1 tm tys2 Hty1)
       = None). {
         eapply match_val_single_alpha_p_none. 2: apply Hmatch1.
@@ -1562,7 +1563,7 @@ Proof.
     destruct p as [p2 t2]. simpl.
     rewrite <- (H _ _ v1 v2 _ Hty1 Hty2 Htm) at 1; auto.
     (*Now need to know [match_val_single] is same - separate lemmas*)
-    destruct ( match_val_single gamma_valid pd vt tys2 p1 (Forall_inv Hpat1)
+    destruct ( match_val_single gamma_valid pd pdf vt tys2 p1 (Forall_inv Hpat1)
     (term_rep v1 tm tys2 Hty1)) eqn : Hmatch1.
     + (*In Some case, need to know how lists relate*)
 
@@ -1571,7 +1572,7 @@ Proof.
         specialize (Hall 0 ltac:(lia)); simpl in Hall. bool_hyps; auto.
       }
       pose proof (alpha_equiv_p_fv_len_full _ _ Hpeq) as Hpfvs.
-      destruct ( match_val_single gamma_valid pd vt tys2 p2 (Forall_inv Hpat2)
+      destruct ( match_val_single gamma_valid pd pdf vt tys2 p2 (Forall_inv Hpat2)
       (term_rep v1 tm tys2 Hty1)) eqn : Hmatch2.
       * assert (A:=Hall). specialize (A 0 ltac:(lia)); simpl in A.
         bool_hyps. rename H1 into Hp. rename H3 into Ht12.
@@ -1671,7 +1672,7 @@ Proof.
         rewrite <- match_val_single_alpha_p_none_iff in Hmatch2.
         rewrite Hmatch2 in Hmatch1. inversion Hmatch1. apply Hpeq.
     + (*In None case, both None, use IH*) 
-      assert (match_val_single gamma_valid pd vt tys2 p2 (Forall_inv Hpat2)
+      assert (match_val_single gamma_valid pd pdf vt tys2 p2 (Forall_inv Hpat2)
       (term_rep v1 tm tys2 Hty1)
       = None). {
         eapply match_val_single_alpha_p_none. 2: apply Hmatch1.
@@ -2362,8 +2363,6 @@ Proof.
   - apply map_snd_combine_nodup; apply NoDup_pat_fv.
   - intros. rewrite map_fst_combine; auto.
 Qed.
-
-Require Import PatternProofs.
 
 Fixpoint shape_p (p1 p2: pattern) :=
   match p1, p2 with
@@ -7155,7 +7154,7 @@ Lemma safe_sub_ts_rep subs t
   (Hty2 : term_has_type gamma t ty):
   term_rep vv (safe_sub_ts subs t) ty Hty1 =
   term_rep (val_with_args pd vt vv (map fst subs)
-      (map_arg_list gamma_valid pd vt pf vv 
+      (map_arg_list gamma_valid pd pdf vt pf vv 
           (map snd subs) (map snd (map fst subs)) 
           (map_snd_fst_len subs) Hall)) t ty Hty2.
 Proof.
@@ -7186,7 +7185,7 @@ Lemma safe_sub_fs_rep subs f
   (Hty2 : formula_typed gamma f):
   formula_rep vv (safe_sub_fs subs f) Hty1 =
   formula_rep (val_with_args pd vt vv (map fst subs)
-      (map_arg_list gamma_valid pd vt pf vv 
+      (map_arg_list gamma_valid pd pdf vt pf vv 
           (map snd subs) (map snd (map fst subs)) 
           (map_snd_fst_len subs) Hall)) f Hty2.
 Proof.
