proofs/proofsystem/MatchSimpl.v
@@ -118,12 +118,13 @@ Proof.
 Qed. 
 
 Lemma match_val_single_matches_none {gamma} (gamma_valid: valid_context gamma)
-  (pd: pi_dom) (vt: val_typevar) (ty: vty) (p: pattern) 
-    (Hty: pattern_has_type gamma p ty) (t: term) (pf: pi_funpred gamma_valid pd) 
+  (pd: pi_dom) (pdf: pi_dom_full gamma pd) 
+    (vt: val_typevar) (ty: vty) (p: pattern) 
+    (Hty: pattern_has_type gamma p ty) (t: term) (pf: pi_funpred gamma_valid pd pdf) 
     (vv: val_vars pd vt) (Hty2: term_has_type gamma t ty):
   matches gamma p t = NoMatch ->
-  match_val_single gamma_valid pd vt ty p Hty
-    (term_rep gamma_valid pd vt pf vv t ty Hty2) = None.
+  match_val_single gamma_valid pd pdf vt ty p Hty
+    (term_rep gamma_valid pd pdf vt pf vv t ty Hty2) = None.
 Proof.
   generalize dependent t. revert Hty. revert ty. induction p; intros; auto;
   try solve[inversion H].
@@ -195,7 +196,7 @@ Proof.
         apply s_params_Nodup.
       }
       subst.
-      erewrite (constrs gamma_valid pd pf m adt f0 m_in a_in c_in).
+      erewrite (constrs gamma_valid pd pdf pf m adt f0 m_in a_in c_in).
       Unshelve. 2: exact (eq_trans (map_length (v_subst vt) vs2) e).
       unfold constr_rep_dom, cast_dom_vty, dom_cast.
       rewrite !scast_scast.
@@ -248,7 +249,7 @@ Proof.
     rewrite Hlenpsl0, Nat.eqb_refl in H0.
     (*Now, we are at the [nested_matches] case, so we need nested induction*)
     match goal with 
-    | |- iter_arg_list ?val ?pd ?l  
+    | |- iter_arg_list ?val ?pd ?pdf ?l  
       (cast_arg_list (sym_sigma_args_map ?vt ?f1 ?vs ?H) ?a) ?ps ?H1 = None =>
       generalize dependent H;
       generalize dependent H1
@@ -262,7 +263,7 @@ Proof.
     simpl in *.
     revert e1.
     simpl_rep_full.
-    erewrite (constrs gamma_valid pd pf m adt f0 Hinctx Hinmut c_in).
+    erewrite (constrs gamma_valid pd pdf pf m adt f0 Hinctx Hinmut c_in).
     Unshelve. 2: exact (eq_trans (map_length (v_subst vt) vs2) e) .
     unfold constr_rep_dom, cast_dom_vty, dom_cast.
     rewrite !scast_scast.
@@ -317,12 +318,12 @@ Qed.
 
 (*See if this is easier*)
 Lemma match_val_single_matches_not_none {gamma} (gamma_valid: valid_context gamma)
-(pd: pi_dom) (vt: val_typevar) (ty: vty) (p: pattern) 
-  (Hty: pattern_has_type gamma p ty) (t: term) (pf: pi_funpred gamma_valid pd) 
+(pd: pi_dom) (pdf: pi_dom_full gamma pd) (vt: val_typevar) (ty: vty) (p: pattern) 
+  (Hty: pattern_has_type gamma p ty) (t: term) (pf: pi_funpred gamma_valid pd pdf) 
   (vv: val_vars pd vt) (Hty2: term_has_type gamma t ty) subs:
 matches gamma p t = Matches subs ->
-match_val_single gamma_valid pd vt ty p Hty
-  (term_rep gamma_valid pd vt pf vv t ty Hty2) <> None.
+match_val_single gamma_valid pd pdf vt ty p Hty
+  (term_rep gamma_valid pd pdf vt pf vv t ty Hty2) <> None.
 Proof.
   generalize dependent t. revert Hty. revert ty. revert subs. induction p; intros; auto;
   try solve[discriminate].
@@ -404,7 +405,7 @@ Proof.
         apply s_params_Nodup.
       }
       subst.
-      erewrite (constrs gamma_valid pd pf m adt f0 Hinctx Hinmut c_in).
+      erewrite (constrs gamma_valid pd pdf pf m adt f0 Hinctx Hinmut c_in).
       Unshelve. 2: exact (eq_trans (map_length (v_subst vt) vs2) e).
       unfold constr_rep_dom, cast_dom_vty, dom_cast.
       rewrite !scast_scast.
@@ -436,7 +437,7 @@ Proof.
     }
     (*Now, we are at the [nested_matches] case, so we need nested induction*)
     match goal with 
-    | |- iter_arg_list ?val ?pd ?l  
+    | |- iter_arg_list ?val ?pd ?pdf ?l  
       (cast_arg_list (sym_sigma_args_map ?vt ?f1 ?vs ?H) ?a) ?ps ?H1 <> None =>
       generalize dependent H;
       generalize dependent H1
@@ -451,7 +452,7 @@ Proof.
     simpl in *.
     revert e0.
     simpl_rep_full.
-    erewrite (constrs gamma_valid pd pf m adt f0 Hinctx Hinmut c_in).
+    erewrite (constrs gamma_valid pd pdf pf m adt f0 Hinctx Hinmut c_in).
     Unshelve. 2: exact (eq_trans (map_length (v_subst vt) vs2) e) .
     unfold constr_rep_dom, cast_dom_vty, dom_cast.
     rewrite !scast_scast.
@@ -524,26 +525,26 @@ Proof.
   inversion H; simpl; auto; f_equal; auto.
 Qed.
 
-(*No, I think we should do it in 2 pieces:
+(*Do it in 2 pieces:
   first, if we have l and l1, they have the relation.
   Then, if [match_val_single] is None, matches is None or
     DontKnow (or can do for Some)*)
 
 (*And the some case*)
 Lemma match_val_single_matches_some {gamma} (gamma_valid: valid_context gamma)
-  (pd: pi_dom) (vt: val_typevar) (ty: vty) (p: pattern) 
-    (Hty: pattern_has_type gamma p ty) (t: term) (pf: pi_funpred gamma_valid pd) 
+  (pd: pi_dom) (pdf: pi_dom_full gamma pd) (vt: val_typevar) (ty: vty) (p: pattern) 
+    (Hty: pattern_has_type gamma p ty) (t: term) (pf: pi_funpred gamma_valid pd pdf) 
     (vv: val_vars pd vt) (Hty2: term_has_type gamma t ty)
     (l: list (vsymbol * term)) l1:
   matches gamma p t = Matches l ->
-  match_val_single gamma_valid pd vt ty p Hty
-  (term_rep gamma_valid pd vt pf vv t ty Hty2) = Some l1 ->
+  match_val_single gamma_valid pd pdf vt ty p Hty
+  (term_rep gamma_valid pd pdf vt pf vv t ty Hty2) = Some l1 ->
   map fst l1 = map fst l /\
   Forall
-    (fun x : {x : sort & domain (dom_aux pd) x} * term =>
+    (fun x : {x : sort & domain pd x} * term =>
      exists ty1 Hty1 (Heq: v_subst vt ty1 = projT1 (fst x)),
        projT2 (fst x) =
-       dom_cast (dom_aux pd) Heq (term_rep gamma_valid pd vt pf vv (snd x) ty1 Hty1))
+       dom_cast pd Heq (term_rep gamma_valid pd pdf vt pf vv (snd x) ty1 Hty1))
     (combine (map snd l1) (map snd l)).
 Proof.
   generalize dependent t. revert Hty. revert ty.
@@ -600,7 +601,7 @@ Proof.
     (*rewrite Hlenpsl0, Nat.eqb_refl in H0.*)
     (*Now, we are at the [nested_matches] case, so we need nested induction*)
     match goal with 
-    | |- iter_arg_list ?val ?pd ?l  
+    | |- iter_arg_list ?val ?pd ?pdf ?l  
       (cast_arg_list (sym_sigma_args_map ?vt ?f1 ?vs ?H) ?a) ?ps ?H1 = Some ?x -> _ =>
       generalize dependent H;
       generalize dependent H1
@@ -614,7 +615,7 @@ Proof.
     simpl in *.
     revert e0.
     simpl_rep_full.
-    erewrite (constrs gamma_valid pd pf m adt f0 Hinctx Hinmut c_in).
+    erewrite (constrs gamma_valid pd pdf pf m adt f0 Hinctx Hinmut c_in).
     Unshelve. 2: exact (eq_trans (map_length (v_subst vt) vs2) e) .
     unfold constr_rep_dom, cast_dom_vty, dom_cast.
     rewrite !scast_scast.
@@ -688,7 +689,7 @@ Proof.
         eapply IHp1. apply Hmatch1. apply Hmatch.
       * (*Here, use previous lemma*) intros Hmatch2.
         exfalso.
-        apply (match_val_single_matches_not_none _ _ _ _ _ _ _ _ _ _ _ 
+        apply (match_val_single_matches_not_none _ _ _ _ _ _ _ _ _ _ _ _ 
           Hmatch1 Hmatch).
   - (*Pbind*)
     simpl in *. revert H0.
@@ -705,26 +706,26 @@ Qed.
 
 (*The combined theorem we want*)
 Lemma match_val_single_matches_some' {gamma} (gamma_valid: valid_context gamma)
-  (pd: pi_dom) (vt: val_typevar) (ty: vty) (p: pattern) 
-    (Hty: pattern_has_type gamma p ty) (t: term) (pf: pi_funpred gamma_valid pd) 
+  (pd: pi_dom) (pdf: pi_dom_full gamma pd) (vt: val_typevar) (ty: vty) (p: pattern) 
+    (Hty: pattern_has_type gamma p ty) (t: term) (pf: pi_funpred gamma_valid pd pdf) 
     (vv: val_vars pd vt) (Hty2: term_has_type gamma t ty)
     (l: list (vsymbol * term)):
   matches gamma p t = Matches l ->
 
   exists l1,
-  match_val_single gamma_valid pd vt ty p Hty
-    (term_rep gamma_valid pd vt pf vv t ty Hty2) = Some l1 /\
+  match_val_single gamma_valid pd pdf vt ty p Hty
+    (term_rep gamma_valid pd pdf vt pf vv t ty Hty2) = Some l1 /\
   map fst l1 = map fst l /\
   Forall
-    (fun x : {x : sort & domain (dom_aux pd) x} * term =>
+    (fun x : {x : sort & domain pd x} * term =>
      exists ty1 Hty1 (Heq: v_subst vt ty1 = projT1 (fst x)),
        projT2 (fst x) =
-       dom_cast (dom_aux pd) Heq (term_rep gamma_valid pd vt pf vv (snd x) ty1 Hty1))
+       dom_cast pd Heq (term_rep gamma_valid pd pdf vt pf vv (snd x) ty1 Hty1))
     (combine (map snd l1) (map snd l)).
 Proof.
   intros.
-  destruct (match_val_single gamma_valid pd vt ty p Hty
-  (term_rep gamma_valid pd vt pf vv t ty Hty2)) eqn : Hmatch.
+  destruct (match_val_single gamma_valid pd pdf vt ty p Hty
+  (term_rep gamma_valid pd pdf vt pf vv t ty Hty2)) eqn : Hmatch.
   - exists l0. split; auto.
     eapply match_val_single_matches_some.
     apply H. apply Hmatch.
@@ -769,11 +770,11 @@ with simpl_match_f gamma (f: formula) : formula :=
   end.
 
 Lemma term_rep_eq {gamma: context} (gamma_valid: valid_context gamma)
-(pd: pi_dom) (vt: val_typevar) (pf: pi_funpred gamma_valid pd) (vv: val_vars pd vt)
+(pd: pi_dom) pdf (vt: val_typevar) (pf: pi_funpred gamma_valid pd pdf) (vv: val_vars pd vt)
 (t1 t2: term) ty (Hty1: term_has_type gamma t1 ty) (Hty2: term_has_type gamma t2 ty):
 t1 = t2 ->
-term_rep gamma_valid pd vt pf vv t1 ty Hty1 =
-term_rep gamma_valid pd vt pf vv t2 ty Hty2.
+term_rep gamma_valid pd pdf vt pf vv t1 ty Hty1 =
+term_rep gamma_valid pd pdf vt pf vv t2 ty Hty2.
 Proof. intros. subst. apply term_rep_irrel. Qed.
 
 
@@ -842,25 +843,26 @@ Qed.
     multiple substitution)*)
 
 Lemma extend_val_with_args_eq {gamma} (gamma_valid: valid_context gamma)
-  (pd: pi_dom) (vt: val_typevar) (pf: pi_funpred gamma_valid pd)
+  (pd: pi_dom) (pdf: pi_dom_full gamma pd) (vt: val_typevar) 
+  (pf: pi_funpred gamma_valid pd pdf)
   (vv: val_vars pd vt)
-  (l1: list (vsymbol * {s : sort & domain (dom_aux pd) s}))
+  (l1: list (vsymbol * {s : sort & domain pd s}))
   (l2: list (vsymbol * term))
   (Hfst: map fst l1 = map fst l2)
   (Hnodup: NoDup (map fst l1))
   (Hsnd: Forall
-    (fun x : {x : sort & domain (dom_aux pd) x} * term =>
+    (fun x : {x : sort & domain pd x} * term =>
     exists
       (ty : vty) (Hty : term_has_type gamma (snd x) ty) 
     (Heq : v_subst vt ty = projT1 (fst x)),
       projT2 (fst x) =
-      dom_cast (dom_aux pd) Heq (term_rep gamma_valid pd vt pf vv (snd x) ty Hty))
+      dom_cast pd Heq (term_rep gamma_valid pd pdf vt pf vv (snd x) ty Hty))
     (combine (map snd l1) (map snd l2)))
   (Hall: Forall (fun x : term * vty => term_has_type gamma (fst x) (snd x))
     (combine (map snd l2) (map snd (map fst l2)))):
   forall x, 
     (val_with_args pd vt vv (map fst l2)
-    (map_arg_list gamma_valid pd vt pf vv (map snd l2) (map snd (map fst l2))
+    (map_arg_list gamma_valid pd pdf vt pf vv (map snd l2) (map snd (map fst l2))
       (map_snd_fst_len l2) Hall)) x =
   (extend_val_with_list pd vt vv l1) x.
 Proof.
@@ -878,7 +880,7 @@ Proof.
   assert (Hleneq: length l1 = length l2). {
     rewrite <- (map_length fst), Hfst, map_length; auto.
   }
-  assert (d: {s : sort & domain (dom_aux pd) s}). {
+  assert (d: {s : sort & domain pd s}). {
     exists s_int. apply dom_int.
   }
   destruct (In_nth _ _ (vs_d, d) Hinsd) as [i [Hi Hxsd]].
@@ -940,7 +942,7 @@ Proof.
   | |- context [dom_cast ?d ?H ?x ] => generalize dependent H
   end.
   repeat match goal with
-  | |- context [term_rep ?g ?pd ?vt ?of ?vv ?t ?ty ?Hty] =>
+  | |- context [term_rep ?g ?pd ?pdf ?vt ?of ?vv ?t ?ty ?Hty] =>
     generalize dependent Hty
   end.
   rewrite !map_map, !map_nth_inbound with (d2:=(vs_d, tm_d)); try lia.
@@ -951,18 +953,19 @@ Proof.
 Qed.
 
 Theorem simpl_match_rep {gamma: context} (gamma_valid: valid_context gamma)
-  (pd: pi_dom) (vt: val_typevar) (pf: pi_funpred gamma_valid pd)
+  (pd: pi_dom) (pdf: pi_dom_full gamma pd) (vt: val_typevar) 
+  (pf: pi_funpred gamma_valid pd pdf)
   (t: term) (f: formula):
   (forall (vv: val_vars pd vt) (ty: vty) 
     (Hty1: term_has_type gamma (simpl_match_t gamma t) ty)
     (Hty2: term_has_type gamma t ty),
-    term_rep gamma_valid pd vt pf vv (simpl_match_t gamma t) ty Hty1 =
-    term_rep gamma_valid pd vt pf vv t ty Hty2) /\
+    term_rep gamma_valid pd pdf vt pf vv (simpl_match_t gamma t) ty Hty1 =
+    term_rep gamma_valid pd pdf vt pf vv t ty Hty2) /\
   (forall (vv: val_vars pd vt)
     (Hty1: formula_typed gamma (simpl_match_f gamma f))
     (Hty2: formula_typed gamma f),
-    formula_rep gamma_valid pd vt pf vv (simpl_match_f gamma f) Hty1 =
-    formula_rep gamma_valid pd vt pf vv f Hty2).
+    formula_rep gamma_valid pd pdf vt pf vv (simpl_match_f gamma f) Hty1 =
+    formula_rep gamma_valid pd pdf vt pf vv f Hty2).
 Proof.
   revert t f; apply term_formula_ind; simpl; intros; try solve[apply term_rep_irrel];
   try solve[apply fmla_rep_irrel].
@@ -996,8 +999,8 @@ Proof.
     {(*if DontKnow, trivial*) contradiction. }
     + (*Case 1: None - we show that [match_val_single] gives None*)
       destruct a as [p1 t1]; simpl in *.
-      assert (match_val_single gamma_valid pd vt v p1 (Forall_inv Hpat2)
-        (term_rep gamma_valid pd vt pf vv tm v Hty2) = None).
+      assert (match_val_single gamma_valid pd pdf vt v p1 (Forall_inv Hpat2)
+        (term_rep gamma_valid pd pdf vt pf vv tm v Hty2) = None).
       { 
         apply match_val_single_matches_none; auto.
       }
@@ -1006,12 +1009,12 @@ Proof.
       destruct a as [p1 t1]; simpl in *. intros.
       (*Let's see lemma*)
       assert (exists l1,
-        match_val_single gamma_valid pd vt v p1 (Forall_inv Hpat2)
-          (term_rep gamma_valid pd vt pf vv tm v Hty2) = Some l1 /\
+        match_val_single gamma_valid pd pdf vt v p1 (Forall_inv Hpat2)
+          (term_rep gamma_valid pd pdf vt pf vv tm v Hty2) = Some l1 /\
         map fst l1 = map fst l /\
         Forall (fun x => exists ty Hty Heq ,
-          projT2 (fst x) = dom_cast (dom_aux pd) Heq 
-            (term_rep gamma_valid pd vt pf vv (snd x) ty Hty) 
+          projT2 (fst x) = dom_cast pd Heq 
+            (term_rep gamma_valid pd pdf vt pf vv (snd x) ty Hty) 
         ) (combine (map snd l1) (map snd l))
       )  .
       {
@@ -1028,7 +1031,7 @@ Proof.
       }
       assert (Hnodup: NoDup (map fst l)). {
         rewrite <- Hfstl1.
-        apply (match_val_single_nodup _ _ _ _ _ _ _ Hmatch).
+        apply (match_val_single_nodup _ _ _ _ _ _ _ _ Hmatch).
       }
       erewrite safe_sub_ts_rep; auto.
       Unshelve.
@@ -1052,9 +1055,9 @@ Proof.
     rewrite Forall_forall in H; apply H. apply nth_In; auto.
   - (*Fquant*)
     assert (Hd: forall d,
-    formula_rep gamma_valid pd vt pf (substi pd vt vv v d) (simpl_match_f gamma f)
+    formula_rep gamma_valid pd pdf vt pf (substi pd vt vv v d) (simpl_match_f gamma f)
     (typed_quant_inv Hty1) =
-    formula_rep gamma_valid pd vt pf (substi pd vt vv v d) f (typed_quant_inv Hty2)).
+    formula_rep gamma_valid pd pdf vt pf (substi pd vt vv v d) f (typed_quant_inv Hty2)).
     {
       intros d. apply H.
     }
@@ -1088,8 +1091,8 @@ Proof.
     {(*if DontKnow, trivial*) contradiction. }
     + (*Case 1: None - we show that [match_val_single] gives None*)
       destruct a as [p1 t1]; simpl in *.
-      assert (match_val_single gamma_valid pd vt v p1 (Forall_inv Hpat2)
-        (term_rep gamma_valid pd vt pf vv tm v Hty2) = None).
+      assert (match_val_single gamma_valid pd pdf vt v p1 (Forall_inv Hpat2)
+        (term_rep gamma_valid pd pdf vt pf vv tm v Hty2) = None).
       { 
         apply match_val_single_matches_none; auto.
       }
@@ -1098,12 +1101,12 @@ Proof.
       destruct a as [p1 t1]; simpl in *. intros.
       (*Let's see lemma*)
       assert (exists l1,
-        match_val_single gamma_valid pd vt v p1 (Forall_inv Hpat2)
-          (term_rep gamma_valid pd vt pf vv tm v Hty2) = Some l1 /\
+        match_val_single gamma_valid pd pdf vt v p1 (Forall_inv Hpat2)
+          (term_rep gamma_valid pd pdf vt pf vv tm v Hty2) = Some l1 /\
         map fst l1 = map fst l /\
         Forall (fun x => exists ty Hty Heq ,
-          projT2 (fst x) = dom_cast (dom_aux pd) Heq 
-            (term_rep gamma_valid pd vt pf vv (snd x) ty Hty) 
+          projT2 (fst x) = dom_cast pd Heq 
+            (term_rep gamma_valid pd pdf vt pf vv (snd x) ty Hty) 
         ) (combine (map snd l1) (map snd l))
       )  .
       {
@@ -1120,7 +1123,7 @@ Proof.
       }
       assert (Hnodup: NoDup (map fst l)). {
         rewrite <- Hfstl1.
-        apply (match_val_single_nodup _ _ _ _ _ _ _ Hmatch).
+        apply (match_val_single_nodup _ _ _ _ _ _ _ _ Hmatch).
       }
       erewrite safe_sub_fs_rep; auto.
       Unshelve.
@@ -1134,11 +1137,11 @@ Proof.
 Qed.
 
 Definition simpl_match_t_rep {gamma} (gamma_valid: valid_context gamma)
-  pd vt pf vv t :=
-  (proj_tm (simpl_match_rep gamma_valid pd vt pf) t) vv.
+  pd pdf vt pf vv t :=
+  (proj_tm (simpl_match_rep gamma_valid pd pdf vt pf) t) vv.
 Definition simpl_match_f_rep {gamma} (gamma_valid: valid_context gamma)
-  pd vt pf vv f :=
-  (proj_fmla (simpl_match_rep gamma_valid pd vt pf) f) vv.
+  pd pdf vt pf vv f :=
+  (proj_fmla (simpl_match_rep gamma_valid pd pdf vt pf) f) vv.
 
 (*Last piece: typing*)
 Lemma simpl_match_ty gamma t f:
